@prefix xsd: <http://www.w3.org/2001/XMLSchema#> .
@prefix owl: <http://www.w3.org/2002/07/owl#> .
@prefix rdf: <http://www.w3.org/1999/02/22-rdf-syntax-ns#> .
@prefix rdfs: <http://www.w3.org/2000/01/rdf-schema#> .
@prefix skos: <http://www.w3.org/2004/02/skos/core#> .
@prefix foaf: <http://xmlns.com/foaf/0.1/> .
@prefix pav: <http://purl.org/pav/> .
@prefix prov: <http://www.w3.org/ns/prov#> .
@prefix org: <http://www.w3.org/ns/org#> .
@prefix dcat: <http://www.w3.org/ns/dcat#> .
@prefix dc: <http://purl.org/dc/elements/1.1/> .
@prefix dcterms: <http://purl.org/dc/terms/> .
@prefix voaf: <http://purl.org/vocommons/voaf#> .
@prefix vann: <http://purl.org/vocab/vann/> .
@prefix cc: <http://creativecommons.org/ns#> .
@prefix coos: <http://id.unece.org/def/coos#> .


#################################################################
# Ontology
#################################################################

<http://id.unece.org/def/coos> a owl:Ontology, voaf:Vocabulary ;
    dc:title "COOS: a core ontology for Official Statistics"@en , "COOS : une ontologie centrale pour la Statistique Officielle"@fr , "COOS: Una ontología básica para las Estadísticas Oficiales"@es ;
    dc:contributor "Guillaume Duffes" , "Dan Gillman" , "Flavio Rizzolo" , "Francine Kalonji", "Juan Muñoz" , "Florian Vucko" ;
    dc:creator "Franck Cotton" ;
    vann:preferredNamespacePrefix "coos" ;
    vann:preferredNamespaceUri <http://id.unece.org/def/coos#> ;
    dc:rights "Copyright © 2021 Unece" ;
    cc:license <http://creativecommons.org/licenses/by/4.0/> ;
    voaf:classNumber "27"^^xsd:integer ;
    voaf:propertyNumber "3"^^xsd:integer ;
    owl:versionInfo "Version 0.1 - 2019-04-04" , "Version 0.3 - 2019-07-02" , "Version 0.4 - 2019-08-29" , "Version 0.5 - 2021-05-03" , "Version 0.6 - 2021-06-30" .


#################################################################
# Classes
#################################################################

# Classes related to the 'activities' domain

coos:Activity a rdfs:Class , owl:Class ;
    rdfs:label "Activity"@en , "Activité"@fr, "Actividad"@es ;
    rdfs:comment "Activity that a statistical organization does."@en , "Activité réalisée par une organisation statistique."@en ;
    skos:definition "Activity that a statistical organization does."@en , "Activité réalisée par une organisation statistique."@en ;
    rdfs:subClassOf skos:Concept , prov:Activity ;
    rdfs:isDefinedBy <http://id.unece.org/def/coos> .

coos:ActivityArea a rdfs:Class , owl:Class ;
    rdfs:label "Activity area"@en , "Secteur d'activité"@fr , "Área de actividad"@es ;
    rdfs:comment "Activity area as defined by the GAMSO."@en , "Secteur d'activité tel que défini par le GAMSO."@fr , "Área de actividad definida conforme a GAMSO."@es ;
    skos:definition "Activity area as defined by the GAMSO."@en , "Secteur d'activité tel que défini par le GAMSO."@fr , "Área de actividad definida conforme a GAMSO."@es ;
    rdfs:subClassOf skos:Concept ;
    rdfs:isDefinedBy <http://id.unece.org/def/coos> .

coos:StatisticalActivity a rdfs:Class , owl:Class ;
    rdfs:label "Statistical activity"@en , "Activité statistique"@fr , "Actividad estadítstica"@es ;
    rdfs:comment "Statistical production activity or activity that directly supports it."@en , "Activité de production statistique ou activité qui la supporte directement."@fr ;
    skos:definition "Statistical production activity or activity that directly supports it"@en , "Activité de production statistique ou activité qui la supporte directement."@fr ;
    rdfs:subClassOf coos:Activity ;
    rdfs:isDefinedBy <http://id.unece.org/def/coos> .

coos:StatisticalProductionActivity a rdfs:Class , owl:Class ;
    rdfs:label "Statistical production activity"@en , "Activité de production statistique"@fr , "Actividad de producción estadística"@es ;
    rdfs:comment "Activity that is conducted as a part of a process to produce statistics"@en , "Activité conduite dans le cadre d'un processus de production de statistiques."@fr ;
    skos:definition "Activity that is conducted as a part of a process to produce statistics"@en , "Activité conduite dans le cadre d'un processus de production de statistiques."@fr , "Actividad de producción estadística cubierta por GSBPM."@es ;
    rdfs:subClassOf coos:StatisticalActivity ;
    rdfs:isDefinedBy <http://id.unece.org/def/coos> .

coos:OverarchingActivity a rdfs:Class , owl:Class ;
    rdfs:label "Overarching statistical production activity"@en , "Activité de production statistique transverse"@fr , "Actividad transversal de producción estadística"@es ;
    rdfs:comment "Activity defined as overarching process by the GSBPM."@en , "Activité définie comme processus transverse par le GSBPM."@fr , "Actividad definida como proceso transversal de acuerdo a GSBPM"@es ;
    skos:definition "Activity defined as overarching process by the GSBPM."@en , "Activité définie comme processus transverse par le GSBPM."@fr , "Actividad definida como proceso transversal de acuerdo a GSBPM"@es ;
    rdfs:subClassOf coos:StatisticalProductionActivity ;
    rdfs:isDefinedBy <http://id.unece.org/def/coos> .

coos:Phase a rdfs:Class , owl:Class ;
    rdfs:label "Statistical production process phase"@en , "Phase du processus de production statistique"@fr , "Fase del proceso de producción estadística"@es ;
    rdfs:comment "Statistical production activity that is conducted at a specific stage of a process as defined by GSBPM phases"@en , "Activité de production statistique conduite à une étape spécifique d'un processus comme défini par les phases du GSBPM."@fr ;
    skos:definition "Statistical production activity that is conducted at a specific stage of a process as defined by GSBPM phases"@en , "Activité de production statistique conduite à une étape spécifique d'un processus comme défini par les phases du GSBPM."@fr ;
    rdfs:subClassOf coos:StatisticalProductionActivity ;
    rdfs:isDefinedBy <http://id.unece.org/def/coos> .

coos:SubProcess a rdfs:Class , owl:Class ;
    rdfs:label "Statistical production sub-process"@en , "Sous-processus de production statistique"@fr , "Subproceso de producción estadística"@es ;
    rdfs:comment "Statistical production activity that is scoped by a given Phase"@en , "Activité de production statistique incluse dans une Phase."@fr ;
    skos:definition "Statistical production activity that is scoped by a given Phase"@en , "Activité de production statistique incluse dans une Phase."@fr ;
    rdfs:subClassOf coos:StatisticalProductionActivity ;
    rdfs:isDefinedBy <http://id.unece.org/def/coos> .

coos:StatisticalProgram a rdfs:Class , owl:Class ;
    rdfs:label "Statistical program"@en , "Programme statistique"@fr , "Programa estadístico"@es ;
    rdfs:comment "As defined by the GSIM."@en , "Tel que défini par le GSIM."@fr , "Tal como está definido en GSIM."@es ;
    skos:definition "As defined by the GSIM."@en , "Tel que défini par le GSIM."@fr , "Tal como está definido en GSIM."@es ;
    rdfs:subClassOf coos:StatisticalActivity , coos:InformationObject ;
    rdfs:isDefinedBy <http://id.unece.org/def/coos> .

coos:StatisticalProgramCycle a rdfs:Class , owl:Class ;
    rdfs:label "Statistical program cycle"@en , "Cycle de programme statistique"@fr , "Ciclo de programa estadístico"@es ;
    rdfs:comment "As defined by the GSIM."@en , "Tel que défini par le GSIM."@fr , "Tal como está definido en GSIM."@es ;
    skos:definition "As defined by the GSIM."@en , "Tel que défini par le GSIM."@fr , "Tal como está definido en GSIM."@es ;
    rdfs:subClassOf coos:StatisticalActivity , coos:InformationObject ;
    rdfs:isDefinedBy <http://id.unece.org/def/coos> .

coos:StatisticalSupportProgram a rdfs:Class , owl:Class ;
    rdfs:label "Statistical support program"@en ;
    rdfs:comment "Corporate-level activity that allows statistical programs to exist and operate."@en ;
    skos:definition "Corporate-level activity that allows statistical programs to exist and operate."@en ;
    rdfs:subClassOf coos:StatisticalActivity , coos:InformationObject ;
    rdfs:isDefinedBy <http://id.unece.org/def/coos> .

coos:Task a rdfs:Class , owl:Class ;
    rdfs:label "Task"@en , "Tâche"@fr , "Tarea"@es ;
    rdfs:comment "Statistical production activity that is scoped by a given GSBPM sub-process"@en , "Activité statistique incluse dans un sous-processus GSBPM donné"@fr , "Actividad estadística limitada por un subproceso dado de GSBPM"@es ;
    skos:definition "Statistical production activity that is scoped by a given GSBPM sub-process"@en , "Activité statistique incluse dans un sous-processus GSBPM donné"@fr , "Actividad estadística limitada por un subproceso dado de GSBPM"@es ;
    skos:scopeNote "Tasks can be more or less fine-grained and form hierarchies"@en , "Les tâches peuvent être de granularité plus ou moins fine et former des hiérarchies"@fr , "Las tareas pueden tener un granularidad mayor o menor y conformar jerarquías"@es ;
    rdfs:subClassOf coos:StatisticalActivity ;
    rdfs:isDefinedBy <http://id.unece.org/def/coos> .

coos:Capability a rdfs:Class , owl:Class ;
    rdfs:label "Capability"@en , "Capacité"@fr , "Capacidad"@es ;
    rdfs:comment "An ability a statistical organization possesses to undertake a specific activity"@en , "Aptitude d'un organisme statistique à entreprendre une activité spécifique"@fr ;
    skos:definition "An ability a statistical organization possesses to undertake a specific activity"@en , "Aptitude d'un organisme statistique à entreprendre une activité spécifique"@fr ;
    skos:scopeNote "A capability is only achieved through the integration of all relevant capability elements (e.g. methods, processes, standards and frameworks, IT systems and people skills)"@en , "Une capacité n'est atteinte que par l'intégration de tous les éléments de capacité pertinents (par exemple, méthodes, processus, normes et cadres, systèmes informatiques et compétences humaines)"@fr ;
    rdfs:subClassOf skos:Concept ;
    rdfs:isDefinedBy <http://id.unece.org/def/coos> .

coos:CoreCapability a rdfs:Class , owl:Class ;
    rdfs:label "Core Capability"@en ;
    rdfs:comment "Capability the organization needs to execute its core business, i.e. the production of statistics."@en , "Capacité dont l'organisation a besoin pour exercer son coeur de métier, c'est-à-dire la production de statistiques."@fr ;
    skos:definition "Capability the organization needs to execute its core business, i.e. the production of statistics."@en , "Capacité dont l'organisation a besoin pour exercer son coeur de métier, c'est-à-dire la production de statistiques."@fr ;
    skos:scopeNote "Core capabilities generally map to phases in GSBPM"@en ;
    rdfs:subClassOf coos:Capability ;
    rdfs:isDefinedBy <http://id.unece.org/def/coos> .

coos:CrossCuttingCapability a rdfs:Class , owl:Class ;
    rdfs:label "Cross-cutting Capability"@en ;
    rdfs:comment "Capability used to formulate and implement the policies that the organization chooses for its internal operations."@en , "Capacité utilisée pour formuler et implémenter les politiques que l'organisation choisit pour ses opérations internes."@fr ;
    rdfs:comment "Capability used to formulate and implement the policies that the organization chooses for its internal operations."@en , "Capacité utilisée pour formuler et implémenter les politiques que l'organisation choisit pour ses opérations internes."@fr ;
    skos:scopeNote "Core capabilities generally map to corporate support activities in GAMSO and overarching processes in GSBPM"@en ;
    rdfs:subClassOf coos:Capability ;
    rdfs:isDefinedBy <http://id.unece.org/def/coos> .

# Additional useful elements from GSIM

coos:InformationObject a rdfs:Class , owl:Class ;
    rdfs:label "Information object"@en , "Objet informationnel"@fr ;
    rdfs:comment "Mother of all classes defined in GSIM."@en , "Mère de toutes les classes définies par le GSIM."@fr , "Madre (raíz) de todas las clases definidas en GSIM."@es ;
    skos:definition "Mother of all classes defined in GSIM."@en , "Mère de toutes les classes définies par le GSIM."@fr , "Madre (raíz) de todas las clases definidas en GSIM."@es ;
    rdfs:isDefinedBy <http://id.unece.org/def/coos> .

coos:StatisticalInformationObject a owl:Class ;
    rdfs:label "Statistical information object"@en , "Objet informationnel statistique"@fr ;
    rdfs:comment "Information object representing statistical information."@en , "Objet informationnel représentant de l'information statistique."@fr ;
    skos:definition "Information object representing statistical information."@en , "Objet informationnel représentant de l'information statistique."@fr ;
    rdfs:isDefinedBy <http://id.unece.org/def/coos> .

coos:StatisticalEntity a rdfs:Class , owl:Class ;
    rdfs:label "Statistical entity"@en , "Entité statistique"@fr , "Entidad estadística"@es ;
    rdfs:comment "Statistical information object which is also an entity in the sense of PROV."@en , "Objet informationnel qui est aussi une entité au sens de PROV."@fr ;
    skos:definition "Statistical information object which is also an entity in the sense of PROV."@en , "Objet informationnel qui est aussi une entité au sens de PROV."@fr ;
    rdfs:subClassOf coos:StatisticalInformationObject , prov:Entity ;
    rdfs:isDefinedBy <http://id.unece.org/def/coos> .

# Classes related to the 'products' domain

coos:StatisticalProduct a rdfs:Class , owl:Class ;
    rdfs:label "Statistical product"@en , "Produit statistique"@fr , "Producto estadístico"@es ;
    rdfs:comment "Corresponds to the GSIM Product."@en , "Correspond au Product GSIM."@fr , "Corresponde a producto en GSIM."@es ;
    skos:definition "Corresponds to the GSIM Product."@en , "Correspond au Product GSIM."@fr , "Corresponde a producto en GSIM."@es ;
    rdfs:subClassOf prov:Entity ;
    rdfs:isDefinedBy <http://id.unece.org/def/coos> .

coos:StatisticalDataset a rdfs:Class , owl:Class ;
    rdfs:label "Statistical dataset"@en , "Jeu de données statistiques"@fr , "Conjunto de datos estadísticos"@es ;
    rdfs:comment "Corresponds to the GSIM Data Set."@en , "Correspond au Data Set GSIM."@fr , "Corresponde a Conjunto de Datos en GSIM"@es ;
    skos:definition "Corresponds to the GSIM Data Set."@en , "Correspond au Data Set GSIM."@fr , "Corresponde a Conjunto de Datos en GSIM"@es ;
    rdfs:subClassOf coos:StatisticalProduct , dcat:Dataset ;
    rdfs:isDefinedBy <http://id.unece.org/def/coos> .

coos:DimensionalDataset a rdfs:Class , owl:Class ;
    rdfs:label "Dimensional dataset"@en ;
    rdfs:comment "Collection of data where each datapoint is uniquely defined by combining one category from each prespecified dimension"@en ;
    skos:definition "Collection of data where each datapoint is uniquely defined by combining one category from each prespecified dimension"@en ;
    rdfs:subClassOf coos:StatisticalDataset ;
    rdfs:isDefinedBy <http://id.unece.org/def/coos> .

coos:GraphDataset a rdfs:Class , owl:Class ;
    rdfs:label "Graph dataset"@en ;
    rdfs:comment "Collection of data organized in a graph-like (including tree-like) structure"@en ;
    skos:definition "Collection of data organized in a graph-like (including tree-like) structure"@en ;
    skos:scopeNote "This includes RDF, property graphs and XML"@en ;
    rdfs:subClassOf coos:StatisticalDataset ;
    rdfs:isDefinedBy <http://id.unece.org/def/coos> .

coos:KeyValueDataset a rdfs:Class , owl:Class ;
    rdfs:label "Key-value dataset"@en ;
    rdfs:comment "Collection of data where each datapoint is paired with a key"@en ;
    skos:definition "Collection of data where each datapoint is paired with a key"@en ;
    rdfs:subClassOf coos:StatisticalDataset ;
    rdfs:isDefinedBy <http://id.unece.org/def/coos> .

coos:RectangularDataset a rdfs:Class , owl:Class ;
    rdfs:label "Rectangular dataset"@en ;
    rdfs:comment "Collection of data where variables are represented with columns"@en ;
    skos:definition "Collection of data where variables are represented with columns"@en ;
    rdfs:subClassOf coos:StatisticalDataset ;
    rdfs:isDefinedBy <http://id.unece.org/def/coos> .

coos:TransposedDataset a rdfs:Class , owl:Class ;
    rdfs:label "Transposed dataset"@en ;
    rdfs:comment "Collection of data where variables are represented with rows"@en ;
    skos:definition "Collection of data where variables are represented with rows"@en ;
    rdfs:subClassOf coos:StatisticalDataset ;
    rdfs:isDefinedBy <http://id.unece.org/def/coos> .

# Classes related to the 'organizations' domain

coos:StatisticalOrganization a rdfs:Class , owl:Class ;
    rdfs:label "Statistical organization"@en , "Organization statistique"@fr , "Organización estadística"@es ;
    rdfs:comment "Organization, or unit within an organization, whose primary role is the production of official statistics."@en ;
    skos:definition "Organization, or unit within an organization, whose primary role is the production of official statistics."@en ;
    rdfs:subClassOf org:Organization , prov:Organization ;
    rdfs:isDefinedBy <http://id.unece.org/def/coos> .

coos:NationalStatisticalInstitute a rdfs:Class , owl:Class ;
    rdfs:label "National statistical institute"@en , "Institut national de statistiques"@fr ,"Instituto nacional de estadística"@es ;
    rdfs:comment "The main producer of official statistics in a country and/or the organization responsible for coordinating all activities related to the development, production, and dissemination of official statistics in the national statistical system."@en ;
    skos:definition "The main producer of official statistics in a country and/or the organization responsible for coordinating all activities related to the development, production, and dissemination of official statistics in the national statistical system."@en ;
    skos:scopeNote "The actual name given to the national statistical office in a country may be National Statistical Institute (NSI), National Bureau of Statistics (NBS), Central Bureau of Statistics (CBS), National Statistical Agency (NSA), Central Statistical Agency (CSA), Central Statistics Agency (CSA), etc."@en ;
    rdfs:subClassOf coos:StatisticalOrganization ;
    owl:disjointWith coos:InternationalAgency ;
    rdfs:isDefinedBy <http://id.unece.org/def/coos> .

coos:InternationalAgency a rdfs:Class , owl:Class ;
    rdfs:label "International agency"@en , "Agence internationale"@fr , "Agencia internacional"@es ;
    rdfs:comment "A body with an international membership, scope, or presence whose primary role is the production of official statistics."@en ;
    skos:definition "A body with an international membership, scope, or presence whose primary role is the production of official statistics."@en ;
    skos:scopeNote "There are many types of international organizations. One way of categorizing them is to distinguish between intergovernmental organizations, supranational organizations and international non-governmental organizations."@en ;
    rdfs:subClassOf coos:StatisticalOrganization ;
    owl:disjointWith coos:NationalStatisticalInstitute ;
    rdfs:isDefinedBy <http://id.unece.org/def/coos> .

#################################################################
# Annotation properties
#################################################################

# No annotation properties in this version of the ontology


#################################################################
# Data properties
#################################################################

# No data properties in this version of the ontology


#################################################################
# Object properties
#################################################################

# Links between GSBPM activities and GAMSO activities

coos:uses a rdfs:Property , owl:ObjectProperty ;
    rdfs:label "uses"@en , "utilise"@fr , "usos"@es ;
    rdfs:comment "To require to perform or function"@en ;
    skos:definition "To require to perform or function"@en ;
    rdfs:domain coos:StatisticalProductionActivity ;
    rdfs:range coos:Activity ;
    owl:inverseOf coos:supports ;
    rdfs:isDefinedBy <http://id.unece.org/def/coos> .

coos:supports a rdfs:Property , owl:ObjectProperty ;
    rdfs:label "supports"@en , "supporte"@fr , "soportes"@es ;
    rdfs:comment "To enable to perform or function."@en ;
    skos:definition "To enable to perform or function."@en ;
    rdfs:domain coos:Activity ;
    rdfs:range coos:StatisticalProductionActivity ;
    owl:inverseOf coos:uses ;
    rdfs:isDefinedBy <http://id.unece.org/def/coos> .

# Characterization of metadata sets

coos:metadataFor a rdfs:Property , owl:ObjectProperty ;
    rdfs:label "metadata for"@en , "métadonnées pour"@fr , "metadatos por"@es ;
    rdfs:comment "Indicates that a dataset contains metadata attached to a given resource"@en ;
    skos:definition "Indicates that a dataset contains metadata attached to a given resource"@en ;
    rdfs:domain coos:StatisticalDataset ;
    rdfs:isDefinedBy <http://id.unece.org/def/coos> .


#################################################################
# Individuals
#################################################################

# The Offical Statistics activity

<http://id.unece.org/activities/officialStatistics> a coos:Activity ;
    skos:notation "OS" ;
    skos:prefLabel "Official Statistics"@en , "Statistique Publique"@fr , "Estadísticas oficiales"@es ;
    skos:inScheme <http://id.unece.org/activities/gamso> ;
    skos:topConceptOf <http://id.unece.org/activities/gamso> ;
    skos:narrower <http://id.unece.org/activities/activityArea/1> , <http://id.unece.org/activities/activityArea/2> , <http://id.unece.org/activities/activityArea/3> , <http://id.unece.org/activities/activityArea/4> .

# The statistical production process

<http://id.unece.org/activities/statisticalProductionProcess> a coos:StatisticalProductionActivity ;
    skos:notation "SPP"	;
    skos:prefLabel "Statistical Production Process"@en , "Processus de Production Statistique"@fr , "Proceso de Producción Estadística"@es ;
    skos:inScheme <http://id.unece.org/activities/gsbpm> ;
    skos:topConceptOf <http://id.unece.org/activities/gsbpm> ;
    skos:exactMatch <http://id.unece.org/activities/activityArea/4> ;
    skos:narrower <http://id.unece.org/activities/phase/1> , <http://id.unece.org/activities/phase/2> , <http://id.unece.org/activities/phase/3> , <http://id.unece.org/activities/phase/4> , <http://id.unece.org/activities/phase/5> , <http://id.unece.org/activities/phase/6> , <http://id.unece.org/activities/phase/7> , <http://id.unece.org/activities/phase/8> .

# The GAMSO activities and activity areas

<http://id.unece.org/activities/activityArea/1> a coos:ActivityArea ;
    skos:notation "1" ;
    skos:prefLabel "Strategy and Leadership"@en , "Estrategia y liderazgo"@es ;
    skos:inScheme <http://id.unece.org/activities/gamso> ;
    skos:broader <http://id.unece.org/activities/officialStatistics> ;
    skos:narrower <http://id.unece.org/activities/activity/1.1> , <http://id.unece.org/activities/activity/1.2> , <http://id.unece.org/activities/activity/1.3> .

<http://id.unece.org/activities/activityArea/2> a coos:ActivityArea ;
    skos:notation "2" ;
    skos:prefLabel "Capability Development"@en , "Desarrollo de capacidades"@es ;
    skos:inScheme <http://id.unece.org/activities/gamso> ;
    skos:broader <http://id.unece.org/activities/officialStatistics> ;
    skos:narrower <http://id.unece.org/activities/activity/2.1> , <http://id.unece.org/activities/activity/2.2> , <http://id.unece.org/activities/activity/2.3> , <http://id.unece.org/activities/activity/2.4> .

<http://id.unece.org/activities/activityArea/3> a coos:ActivityArea ;
    skos:notation "3" ;
    skos:prefLabel "Corporate Support"@en , "Soporte Corporativo"@es ;
    skos:inScheme <http://id.unece.org/activities/gamso> ;
    skos:broader <http://id.unece.org/activities/officialStatistics> ;
    skos:narrower <http://id.unece.org/activities/activity/3.1> , <http://id.unece.org/activities/activity/3.2> , <http://id.unece.org/activities/activity/3.3> , <http://id.unece.org/activities/activity/3.4> , <http://id.unece.org/activities/activity/3.5> , <http://id.unece.org/activities/activity/3.6> , <http://id.unece.org/activities/activity/3.7> , <http://id.unece.org/activities/activity/3.8> , <http://id.unece.org/activities/activity/3.9> , <http://id.unece.org/activities/activity/3.10> .

<http://id.unece.org/activities/activityArea/4> a coos:ActivityArea ;
    skos:notation "4" ;
    skos:prefLabel "Production"@en , "Producción"@es ;
    skos:inScheme <http://id.unece.org/activities/gamso> ;
    skos:broader <http://id.unece.org/activities/officialStatistics> ;
    skos:exactMatch <http://id.unece.org/activities/statisticalProductionProcess> .

<http://id.unece.org/activities/activity/1.1> a coos:Activity ;
    skos:notation "1.1" ;
    skos:prefLabel "Define Vision"@en , "Definir la Visión"@es ;
    skos:inScheme <http://id.unece.org/activities/gamso> ;
    skos:broader <http://id.unece.org/activities/activityArea/1> .

<http://id.unece.org/activities/activity/1.2> a coos:Activity ;
    skos:notation "1.2" ;
    skos:prefLabel "Govern and Lead"@en , "Gobierno y Liderazgo"@es ;
    skos:inScheme <http://id.unece.org/activities/gamso> ;
    skos:broader <http://id.unece.org/activities/activityArea/1> .

<http://id.unece.org/activities/activity/1.3> a coos:Activity ;
    skos:notation "1.3" ;
    skos:prefLabel "Manage Strategic Collaboration and Cooperation"@en , "Administrar la Colaboración y Cooperación Estratégicas"@es ;
    skos:inScheme <http://id.unece.org/activities/gamso> ;
    skos:broader <http://id.unece.org/activities/activityArea/1> .

<http://id.unece.org/activities/activity/2.1> a coos:Activity ;
    skos:notation "2.1" ;
    skos:prefLabel "Plan Capability Improvements"@en , "Planificar Mejoras a las Capacidades"@es ;
    skos:inScheme <http://id.unece.org/activities/gamso> ;
    skos:broader <http://id.unece.org/activities/activityArea/2> .

<http://id.unece.org/activities/activity/2.2> a coos:Activity ;
    skos:notation "2.2" ;
    skos:prefLabel "Develop Capability Improvements"@en , "Desarrollar Mejoras a las Capacidades"@es ;
    skos:inScheme <http://id.unece.org/activities/gamso> ;
    skos:broader <http://id.unece.org/activities/activityArea/2> .

<http://id.unece.org/activities/activity/2.3> a coos:Activity ;
    skos:notation "2.3" ;
    skos:prefLabel "Monitor Capability Improvements"@en , "Monitorear Mejoras a las Capacidades"@es ;
    skos:inScheme <http://id.unece.org/activities/gamso> ;
    skos:broader <http://id.unece.org/activities/activityArea/2> .

<http://id.unece.org/activities/activity/2.4> a coos:Activity ;
    skos:notation "2.4" ;
    skos:prefLabel "Transfer Support of Capability Improvements"@en , "Soporte de la Transferencia a las Mejoras a las Capacidades"@es ;
    skos:inScheme <http://id.unece.org/activities/gamso> ;
    skos:broader <http://id.unece.org/activities/activityArea/2> .

<http://id.unece.org/activities/activity/3.1> a coos:Activity ;
    skos:notation "3.1" ;
    skos:prefLabel "Manage Business Performance and Legislation"@en , "Administrar el Desempeño y Legislación de los Procesos"@es ;
    skos:inScheme <http://id.unece.org/activities/gamso> ;
    skos:broader <http://id.unece.org/activities/activityArea/3> .

<http://id.unece.org/activities/activity/3.2> a coos:Activity , coos:StatisticalActivity ;
    skos:notation "3.2" ;
    skos:prefLabel "Manage Statistical Methodology"@en , "Administrar la Metodología Estadística"@es ;
    skos:inScheme <http://id.unece.org/activities/gamso> ;
    skos:broader <http://id.unece.org/activities/activityArea/3> .

<http://id.unece.org/activities/activity/3.3> a coos:Activity ;
    skos:notation "3.3" ;
    skos:prefLabel "Manage Quality"@en , "Administrar la Calidad"@es ;
    skos:inScheme <http://id.unece.org/activities/gamso> ;
    skos:broader <http://id.unece.org/activities/activityArea/3> ;
    coos:supports <http://id.unece.org/activities/overarchingActivity/0.1> .

<http://id.unece.org/activities/activity/3.4> a coos:Activity ;
    skos:notation "3.4" ;
    skos:prefLabel "Manage Information and Knowledge"@en , "Administrar la Información y el Conocimiento"@es ;
    skos:inScheme <http://id.unece.org/activities/gamso> ;
    skos:broader <http://id.unece.org/activities/activityArea/3> .

<http://id.unece.org/activities/activity/3.5> a coos:Activity ;
    skos:notation "3.5" ;
    skos:prefLabel "Manage Consumers"@en , "Adminitrar los Consumidores"@es ;
    skos:inScheme <http://id.unece.org/activities/gamso> ;
    skos:broader <http://id.unece.org/activities/activityArea/3> .

<http://id.unece.org/activities/activity/3.6> a coos:Activity , coos:StatisticalActivity ;
    skos:notation "3.6" ;
    skos:prefLabel "Manage Data Suppliers"@en , "Administrar a los Proveedores de Datos"@es ;
    skos:inScheme <http://id.unece.org/activities/gamso> ;
    skos:broader <http://id.unece.org/activities/activityArea/3> .

<http://id.unece.org/activities/activity/3.7> a coos:Activity ;
    skos:notation "3.7" ;
    skos:prefLabel "Manage Finances"@en , "Administrar las Finanzas"@es ;
    skos:inScheme <http://id.unece.org/activities/gamso> ;
    skos:broader <http://id.unece.org/activities/activityArea/3> .

<http://id.unece.org/activities/activity/3.8> a coos:Activity ;
    skos:notation "3.8" ;
    skos:prefLabel "Manage Human Resources"@en , "Administrar los Recursos Humanos"@es ;
    skos:inScheme <http://id.unece.org/activities/gamso> ;
    skos:broader <http://id.unece.org/activities/activityArea/3> .

<http://id.unece.org/activities/activity/3.9> a coos:Activity ;
    skos:notation "3.9" ;
    skos:prefLabel "Manage Information Technology (IT)"@en , "Administrar las Tecnologías de la Información (TI)"@es ;
    skos:inScheme <http://id.unece.org/activities/gamso> ;
    skos:broader <http://id.unece.org/activities/activityArea/3> .

<http://id.unece.org/activities/activity/3.10> a coos:Activity ;
    skos:notation "3.10" ;
    skos:prefLabel "Manage Buildings and Physical Space"@en , "Administrar Edificios y Espacios Físicos"@es ;
    skos:inScheme <http://id.unece.org/activities/gamso> ;
    skos:broader <http://id.unece.org/activities/activityArea/3> .

# The GSBPM overarching processes

<http://id.unece.org/activities/overarchingActivity/0.1> a coos:OverarchingActivity ;
    skos:notation "0.1"	;
    skos:prefLabel "Quality Management"@en , "Gestion de la qualité"@fr , "Administración de la Calidad"@es ;
    coos:uses <http://id.unece.org/activities/activity/3.3> .

<http://id.unece.org/activities/overarchingActivity/0.2> a coos:OverarchingActivity ;
    skos:notation "0.2"	;
    skos:prefLabel "Metadata Management"@en , "Gestion des métadonnées"@fr , "Administración de Metadatos"@es .

<http://id.unece.org/activities/overarchingActivity/0.3> a coos:OverarchingActivity ;
    skos:notation "0.3"	;
    skos:prefLabel "Data Management"@en , "Gestion des données"@fr , "Administración de Datos"@es .

# The GSBPM phases and sub-process

<http://id.unece.org/activities/phase/1> a coos:Phase ;
    skos:notation "1" ;
    skos:prefLabel "Specify Needs"@en , "Especificación de Necesidades"@es ;
    skos:inScheme <http://id.unece.org/activities/gsbpm> ;
    skos:broader <http://id.unece.org/activities/statisticalProductionProcess> ;
    skos:narrower <http://id.unece.org/activities/subProcess/1.1> , <http://id.unece.org/activities/subProcess/1.2> , <http://id.unece.org/activities/subProcess/1.3> , <http://id.unece.org/activities/subProcess/1.4> , <http://id.unece.org/activities/subProcess/1.5> , <http://id.unece.org/activities/subProcess/1.6> .

<http://id.unece.org/activities/phase/2> a coos:Phase ;
    skos:notation "2" ;
    skos:prefLabel "Design"@en , "Diseño"@es ;
    skos:inScheme <http://id.unece.org/activities/gsbpm> ;
    skos:broader <http://id.unece.org/activities/statisticalProductionProcess> ;
    skos:narrower <http://id.unece.org/activities/subProcess/2.1> , <http://id.unece.org/activities/subProcess/2.2> , <http://id.unece.org/activities/subProcess/2.3> , <http://id.unece.org/activities/subProcess/2.4> , <http://id.unece.org/activities/subProcess/2.5> , <http://id.unece.org/activities/subProcess/2.6> .

<http://id.unece.org/activities/phase/3> a coos:Phase ;
    skos:notation "3" ;
    skos:prefLabel "Build"@en , "Construcción"@es ;
    skos:inScheme <http://id.unece.org/activities/gsbpm> ;
    skos:broader <http://id.unece.org/activities/statisticalProductionProcess> ;
    skos:narrower <http://id.unece.org/activities/subProcess/3.1> , <http://id.unece.org/activities/subProcess/3.2> , <http://id.unece.org/activities/subProcess/3.3> , <http://id.unece.org/activities/subProcess/3.4> , <http://id.unece.org/activities/subProcess/3.5> , <http://id.unece.org/activities/subProcess/3.6> , <http://id.unece.org/activities/subProcess/3.7> .

<http://id.unece.org/activities/phase/4> a coos:Phase ;
    skos:notation "4" ;
    skos:prefLabel "Collect"@en , "Recolección"@es ;
    skos:inScheme <http://id.unece.org/activities/gsbpm> ;
    skos:broader <http://id.unece.org/activities/statisticalProductionProcess> ;
    skos:narrower <http://id.unece.org/activities/subProcess/4.1> , <http://id.unece.org/activities/subProcess/4.2> , <http://id.unece.org/activities/subProcess/4.3> , <http://id.unece.org/activities/subProcess/4.4> .

<http://id.unece.org/activities/phase/5> a coos:Phase ;
    skos:notation "5" ;
    skos:prefLabel "Process"@en , "Procesamiento"@es ;
    skos:inScheme <http://id.unece.org/activities/gsbpm> ;
    skos:broader <http://id.unece.org/activities/statisticalProductionProcess> ;
    skos:narrower <http://id.unece.org/activities/subProcess/5.1> , <http://id.unece.org/activities/subProcess/5.2> , <http://id.unece.org/activities/subProcess/5.3> , <http://id.unece.org/activities/subProcess/5.4> , <http://id.unece.org/activities/subProcess/5.5> , <http://id.unece.org/activities/subProcess/5.6> , <http://id.unece.org/activities/subProcess/5.7> , <http://id.unece.org/activities/subProcess/5.8> .

<http://id.unece.org/activities/phase/6> a coos:Phase ;
    skos:notation "6" ;
    skos:prefLabel "Analyse"@en , "Analísis"@es ;
    skos:inScheme <http://id.unece.org/activities/gsbpm> ;
    skos:broader <http://id.unece.org/activities/statisticalProductionProcess> ;
    skos:narrower <http://id.unece.org/activities/subProcess/6.1> , <http://id.unece.org/activities/subProcess/6.2> , <http://id.unece.org/activities/subProcess/6.3> , <http://id.unece.org/activities/subProcess/6.4> , <http://id.unece.org/activities/subProcess/6.5> .

<http://id.unece.org/activities/phase/7> a coos:Phase ;
    skos:notation "7" ;
    skos:prefLabel "Disseminate"@en , "Difusión"@es ;
    skos:inScheme <http://id.unece.org/activities/gsbpm> ;
    skos:broader <http://id.unece.org/activities/statisticalProductionProcess> ;
    skos:narrower <http://id.unece.org/activities/subProcess/7.1> , <http://id.unece.org/activities/subProcess/7.2> , <http://id.unece.org/activities/subProcess/7.3> , <http://id.unece.org/activities/subProcess/7.4> , <http://id.unece.org/activities/subProcess/7.5> .

<http://id.unece.org/activities/phase/8> a coos:Phase ;
    skos:notation "8" ;
    skos:prefLabel "Evaluate"@en , "Evaluación"@es ;
    skos:inScheme <http://id.unece.org/activities/gsbpm> ;
    skos:broader <http://id.unece.org/activities/statisticalProductionProcess> ;
    skos:narrower <http://id.unece.org/activities/subProcess/8.1> , <http://id.unece.org/activities/subProcess/8.2> , <http://id.unece.org/activities/subProcess/8.3> .

<http://id.unece.org/activities/subProcess/1.1> a coos:SubProcess ;
    skos:notation "1.1" ;
	skos:prefLabel "Identify needs"@en , "Identificar necesidades"@es ;
    skos:broader <http://id.unece.org/activities/phase/1> .

<http://id.unece.org/activities/subProcess/1.2> a coos:SubProcess ;
    skos:notation "1.2" ;
    skos:prefLabel "Consult and confirm needs"@en , "Consultar y confirmar necesidades"@es ;
    skos:broader <http://id.unece.org/activities/phase/1> .

<http://id.unece.org/activities/subProcess/1.3> a coos:SubProcess ;
    skos:notation "1.3" ;
	skos:prefLabel "Establish output objectives"@en , "Establecer objetivos de salidas"@es ;
    skos:broader <http://id.unece.org/activities/phase/1> .

<http://id.unece.org/activities/subProcess/1.4> a coos:SubProcess ;
    skos:notation "1.4" ;
	skos:prefLabel "Identify concepts"@en , "Identificar conceptos"@es ;
    skos:broader <http://id.unece.org/activities/phase/1> .

<http://id.unece.org/activities/subProcess/1.5> a coos:SubProcess ;
    skos:notation "1.5" ;
    skos:prefLabel "Check data availability"@en , "Revisar la disponibilidad de datos"@es ;
    skos:broader <http://id.unece.org/activities/phase/1> .

<http://id.unece.org/activities/subProcess/1.6> a coos:SubProcess ;
    skos:notation "1.6" ;
    skos:prefLabel "Prepare and submit business case"@en , "Preparar y enviar el caso de negocio"@es;
    skos:broader <http://id.unece.org/activities/phase/1> .

<http://id.unece.org/activities/subProcess/2.1> a coos:SubProcess ;
    skos:notation "2.1" ;
    skos:prefLabel "Design outputs"@en , "Diseñar salidas"@es ;
    skos:broader <http://id.unece.org/activities/phase/2> .

<http://id.unece.org/activities/subProcess/2.2> a coos:SubProcess ;
    skos:notation "2.2" ;
    skos:prefLabel "Design variable descriptions"@en , "Diseñar descripciones de variables"@es ;
    skos:broader <http://id.unece.org/activities/phase/2> .

<http://id.unece.org/activities/subProcess/2.3> a coos:SubProcess ;
    skos:notation "2.3" ;
    skos:prefLabel "Design collection"@en , "Diseñar recolección"@es ;
    skos:broader <http://id.unece.org/activities/phase/2> .

<http://id.unece.org/activities/subProcess/2.4> a coos:SubProcess ;
    skos:notation "2.4" ;
    skos:prefLabel "Design frame and sample"@en , "Diseñar marco y muestra"@es;
    skos:broader <http://id.unece.org/activities/phase/2> .

<http://id.unece.org/activities/subProcess/2.5> a coos:SubProcess ;
    skos:notation "2.5" ;
    skos:prefLabel "Design processing and analysis"@en , "Diseñar procesamiento y análisis"@es ;
    skos:broader <http://id.unece.org/activities/phase/2> .

<http://id.unece.org/activities/subProcess/2.6> a coos:SubProcess ;
    skos:notation "2.6" ;
	skos:prefLabel "Design production systems and workflow"@en , "Diseñar sistemas de producción y flujo de trabajo"@es ;
    skos:broader <http://id.unece.org/activities/phase/2> .

<http://id.unece.org/activities/subProcess/3.1> a coos:SubProcess ;
    skos:notation "3.1" ;
    skos:prefLabel "Reuse or build collection instruments"@en , "Reutilizar o construir instrumentos de recolección"@es ;
    skos:broader <http://id.unece.org/activities/phase/3> .

<http://id.unece.org/activities/subProcess/3.2> a coos:SubProcess ;
    skos:notation "3.2" ;
	skos:prefLabel "Reuse or build analysis components"@en , "Reutilizar o construir componentes de análisis"@es ;
    skos:broader <http://id.unece.org/activities/phase/3> .

<http://id.unece.org/activities/subProcess/3.3> a coos:SubProcess ;
    skos:notation "3.3" ;
	skos:prefLabel "Reuse or build dissemination components"@en , "Reutilizar o construir componentes de difusión"@es ;
    skos:broader <http://id.unece.org/activities/phase/3> .

<http://id.unece.org/activities/subProcess/3.4> a coos:SubProcess ;
    skos:notation "3.4" ;
	skos:prefLabel "Configure workflows"@en , "Configurar flujos de trabajo"@es ;
    skos:broader <http://id.unece.org/activities/phase/3> .

<http://id.unece.org/activities/subProcess/3.5> a coos:SubProcess ;
    skos:notation "3.5" ;
    skos:prefLabel "Test production systems"@en , "Probar sistemas de producción"@es ;
    skos:broader <http://id.unece.org/activities/phase/3> .

<http://id.unece.org/activities/subProcess/3.6> a coos:SubProcess ;
    skos:notation "3.6" ;
    skos:prefLabel "Test statistical business process"@en , "Probar procesos estadísticos"@es ;
    skos:broader <http://id.unece.org/activities/phase/3> .

<http://id.unece.org/activities/subProcess/3.7> a coos:SubProcess ;
    skos:notation "3.7" ;
	skos:prefLabel "Finalise production systems"@en , "Finalizar sistemas de producción"@es ;
	skos:broader <http://id.unece.org/activities/phase/3> .

<http://id.unece.org/activities/subProcess/4.1> a coos:SubProcess ;
    skos:notation "4.1" ;
    skos:prefLabel "Create frame and select sample"@en , "Crear marco y seleccionar muestra"@es ;
    skos:broader <http://id.unece.org/activities/phase/4> .

<http://id.unece.org/activities/subProcess/4.2> a coos:SubProcess ;
    skos:notation "4.2" ;
    skos:prefLabel "Set up collection"@en , "Establecer recolección"@es ;
    skos:broader <http://id.unece.org/activities/phase/4> .

<http://id.unece.org/activities/subProcess/4.3> a coos:SubProcess ;
    skos:notation "4.3" ;
    skos:prefLabel "Run collection"@en , "Ejecutar recolección"@es ;
    skos:broader <http://id.unece.org/activities/phase/4> .

<http://id.unece.org/activities/subProcess/4.4> a coos:SubProcess ;
    skos:notation "4.4" ;
    skos:prefLabel "Finalise collection"@en , "Finalizar recolección"@es ;
    skos:broader <http://id.unece.org/activities/phase/4> .

<http://id.unece.org/activities/subProcess/5.1> a coos:SubProcess ; 
    skos:notation "5.1" ;
    skos:prefLabel "Integrate data"@en , "Integrar datos"@es ;
    skos:broader <http://id.unece.org/activities/phase/5> .

<http://id.unece.org/activities/subProcess/5.2> a coos:SubProcess ;
    skos:notation "5.2" ;
    skos:prefLabel "Classify and code"@en , "Clasificar y codificar"@es ;
    skos:broader <http://id.unece.org/activities/phase/5> .

<http://id.unece.org/activities/subProcess/5.3> a coos:SubProcess ;
    skos:notation "5.3" ;
	skos:prefLabel "Review and validate"@en , "Revisar y validar"@es ;
    skos:broader <http://id.unece.org/activities/phase/5> .

<http://id.unece.org/activities/subProcess/5.4> a coos:SubProcess ;
    skos:notation "5.4" ;
    skos:prefLabel "Edit and impute"@en , "Editar e imputar"@es ;
    skos:broader <http://id.unece.org/activities/phase/5> .

<http://id.unece.org/activities/subProcess/5.5> a coos:SubProcess ;
    skos:notation "5.5" ;
    skos:prefLabel "Derive new variables and units"@en , "Derivar nuevas variables y unidades"@es ;
    skos:broader <http://id.unece.org/activities/phase/5> .

<http://id.unece.org/activities/subProcess/5.6> a coos:SubProcess ;
    skos:notation "5.6" ;
    skos:prefLabel "Calculate weights"@en , "Calcular pesos"@es ;
    skos:broader <http://id.unece.org/activities/phase/5> .

<http://id.unece.org/activities/subProcess/5.7> a coos:SubProcess ;
    skos:notation "5.7" ;
    skos:prefLabel "Calculate aggregates"@en , "Calcular agregados"@es ;
    skos:broader <http://id.unece.org/activities/phase/5> .

<http://id.unece.org/activities/subProcess/5.8> a coos:SubProcess ;
    skos:notation "5.8" ;
    skos:prefLabel "Finalise data files"@en , "Finalizar archivos de datos"@es ;
    skos:broader <http://id.unece.org/activities/phase/5> .

<http://id.unece.org/activities/subProcess/6.1> a coos:SubProcess ;
    skos:notation "6.1" ;
    skos:prefLabel "Prepare draft outputs"@en , "Preparar salidas preliminares"@es ;
    skos:broader <http://id.unece.org/activities/phase/6> .

<http://id.unece.org/activities/subProcess/6.2> a coos:SubProcess ;
    skos:notation "6.2" ;
    skos:prefLabel "Validate outputs"@en , "Validar salidas"@es ;
    skos:broader <http://id.unece.org/activities/phase/6> .

<http://id.unece.org/activities/subProcess/6.3> a coos:SubProcess ;
    skos:notation "6.3" ;
    skos:prefLabel "Interpret and explain outputs"@en , "Interpretar y explicar salidas"@es ;
    skos:broader <http://id.unece.org/activities/phase/6> .

<http://id.unece.org/activities/subProcess/6.4> a coos:SubProcess ;
    skos:notation "6.4" ;
    skos:prefLabel "Apply disclosure control"@en , "Aplicar control de divulgación"@es ;
    skos:broader <http://id.unece.org/activities/phase/6> .

<http://id.unece.org/activities/subProcess/6.5> a coos:SubProcess ;
    skos:notation "6.5" ;
    skos:prefLabel "Finalise outputs"@en , "Finalizar salidas"@es ;
    skos:broader <http://id.unece.org/activities/phase/6> .

<http://id.unece.org/activities/subProcess/7.1> a coos:SubProcess ;
    skos:notation "7.1" ;
    skos:prefLabel "Update output systems"@en , "Actualizar sistemas de salida"@es ;
    skos:broader <http://id.unece.org/activities/phase/7> .

<http://id.unece.org/activities/subProcess/7.2> a coos:SubProcess ;
    skos:notation "7.2" ;
    skos:prefLabel "Produce dissemination products"@en , "Producir productos de difusión"@es ;
    skos:broader <http://id.unece.org/activities/phase/7> .

<http://id.unece.org/activities/subProcess/7.3> a coos:SubProcess ;
    skos:notation "7.3" ;
    skos:prefLabel "Manage release of dissemination products"@en , "Administrar la publicación de productos de difusión"@es ;
    skos:broader <http://id.unece.org/activities/phase/7> .

<http://id.unece.org/activities/subProcess/7.4> a coos:SubProcess ;
    skos:notation "7.4" ;
    skos:prefLabel "Promote dissemination products"@en , "Promover los productos de difusión"@es ;
    skos:broader <http://id.unece.org/activities/phase/7> .

<http://id.unece.org/activities/subProcess/7.5> a coos:SubProcess ;
    skos:notation "7.5" ;
    skos:prefLabel "Manage user support"@en , "Administrar el soporte al usuario"@es ;
    skos:broader <http://id.unece.org/activities/phase/7> .

<http://id.unece.org/activities/subProcess/8.1> a coos:SubProcess ;
    skos:notation "8.1" ;
    skos:prefLabel "Gather evaluation inputs"@en , "Obtener entradas de evaluación"@es ;
    skos:broader <http://id.unece.org/activities/phase/8> .

<http://id.unece.org/activities/subProcess/8.2> a coos:SubProcess ;
    skos:notation "8.2" ;
    skos:prefLabel "Conduct evaluation"@en , "Conducir la evaluación"@es ;
    skos:broader <http://id.unece.org/activities/phase/8> .

<http://id.unece.org/activities/subProcess/8.2> a coos:SubProcess ;
    skos:notation "8.3" ;
    skos:prefLabel "Agree an action plan"@en , "Acordar un plan de acción"@es ;
    skos:broader <http://id.unece.org/activities/phase/8> .

# The GAMSO/GSBPM concept schemes (see issue 2)

<http://id.unece.org/activities/gamso> a skos:ConceptScheme ;
    skos:prefLabel "Generic Activity Model for Statistical Organisations"@en , "Modelo Genérico de Actividades para las Organizaciones Estadísticas"@es ;
    skos:notation "GAMSO" ;
    pav:version  "v1.2" ;
    foaf:homePage <https://statswiki.unece.org/display/GAMSO/GAMSO+v1.2> ;
    dcterms:hasPart <http://id.unece.org/activities/gsbpm> ;
    skos:hasTopConcept <http://id.unece.org/activities/officialStatistics> .

<http://id.unece.org/activities/gsbpm> a skos:ConceptScheme ;
    skos:prefLabel "Generic Statistical Business Process Model"@en , "Modelo Genérico del Proceso Estadístico"@es;
    skos:notation "GSBPM" ;
    pav:version  "v5.1" ;
    foaf:homePage <https://statswiki.unece.org/display/GSBPM/GSBPM+v5.1> ;
    dcterms:isPartOf <http://id.unece.org/activities/gamso> ;
    skos:hasTopConcept <http://id.unece.org/activities/statisticalProductionProcess> .
